{
"cells": [
{"cell_type":    "code", "execution_count":null, "metadata":{}, "source":["%%html\n<link href=\"http://mathbook.pugetsound.edu/beta/mathbook-content.css\" rel=\"stylesheet\" type=\"text/css\" />\n<link href=\"https://aimath.org/mathbook/mathbook-add-on.css\" rel=\"stylesheet\" type=\"text/css\" />\n<style>.subtitle {font-size:medium; display:block}</style>\n<link href=\"https://fonts.googleapis.com/css?family=Open+Sans:400,400italic,600,600italic\" rel=\"stylesheet\" type=\"text/css\" />\n<link href=\"https://fonts.googleapis.com/css?family=Inconsolata:400,700&subset=latin,latin-ext\" rel=\"stylesheet\" type=\"text/css\" /><!-- Hide this cell. -->\n<script>\nvar cell = $(\".container .cell\").eq(0), ia = cell.find(\".input_area\")\nif (cell.find(\".toggle-button\").length == 0) {\nia.after(\n    $('<button class=\"toggle-button\">Toggle hidden code</button>').click(\n        function (){ ia.toggle() }\n        )\n    )\nia.hide()\n}\n</script>\n"], "outputs":[]},
{"cell_type":"markdown", "metadata":{}, "source":["**Important:** to view this notebook properly you will need to execute the cell above, which assumes you have an Internet connection.  It should already be selected, or place your cursor anywhere above to select.  Then press the \"Run\" button in the menu bar above (the right-pointing arrowhead), or press Shift-Enter on your keyboard."]},
{"cell_type":"markdown", "metadata":{}, "source":["$\\newcommand{\\identity}{\\mathrm{id}}\n\\newcommand{\\notdivide}{{\\not{\\mid}}}\n\\newcommand{\\notsubset}{\\not\\subset}\n\\newcommand{\\lcm}{\\operatorname{lcm}}\n\\newcommand{\\gf}{\\operatorname{GF}}\n\\newcommand{\\inn}{\\operatorname{Inn}}\n\\newcommand{\\aut}{\\operatorname{Aut}}\n\\newcommand{\\Hom}{\\operatorname{Hom}}\n\\newcommand{\\cis}{\\operatorname{cis}}\n\\newcommand{\\chr}{\\operatorname{char}}\n\\newcommand{\\Null}{\\operatorname{Null}}\n\\newcommand{\\lt}{<}\n\\newcommand{\\gt}{>}\n\\newcommand{\\amp}{&}\n$"]},
{"cell_type":"markdown", "metadata":{}, "source":["<div class=\"mathbook-content\"><h2 class=\"heading hide-type\" alt=\"Section 2.1 Mathematical Induction\"><span class=\"type\">Section</span><span class=\"codenumber\">2.1</span><span class=\"title\">Mathematical Induction</span></h2><a href=\"section-math-induction.ipynb\" class=\"permalink\">Â¶</a></div>"]},
{"cell_type":"markdown", "metadata":{}, "source":["<div class=\"mathbook-content\"><p id=\"p-246\">Suppose we wish to show that</p><div class=\"displaymath\">\n\\begin{equation*}\n1 + 2 + \\cdots + n = \\frac{n(n + 1)}{2}\n\\end{equation*}\n</div><p>for any natural number $n\\text{.}$ This formula is easily  verified for small numbers such as $n = 1\\text{,}$ 2, 3, or 4, but it is impossible to verify for all natural numbers on a case-by-case basis.  To prove the formula true in general, a more generic method is required.</p></div>"]},
{"cell_type":"markdown", "metadata":{}, "source":["<div class=\"mathbook-content\"><p id=\"p-247\">Suppose we have verified the equation for the first $n$ cases.  We will attempt to show that we can generate the formula for the $(n + 1)$th case from this knowledge.  The formula is true for $n = 1$ since</p><div class=\"displaymath\">\n\\begin{equation*}\n1 = \\frac{1(1 + 1)}{2}.\n\\end{equation*}\n</div><p>If we have verified the first $n$ cases, then</p><div class=\"displaymath\">\n\\begin{align*}\n1 + 2 + \\cdots + n + (n + 1) & = \\frac{n(n + 1)}{2} + n + 1\\\\\n& = \\frac{n^2 + 3n + 2}{2}\\\\\n& = \\frac{(n + 1)[(n + 1) + 1]}{2}.\n\\end{align*}\n</div></div>"]},
{"cell_type":"markdown", "metadata":{}, "source":["<div class=\"mathbook-content\"><p id=\"p-248\">This is exactly the formula for the $(n + 1)$th case.</p></div>"]},
{"cell_type":"markdown", "metadata":{}, "source":["<div class=\"mathbook-content\"><p id=\"p-249\">This method of proof is known as <dfn class=\"terminology\">mathematical induction</dfn>.  Instead of attempting to verify a statement about some subset $S$ of the positive integers ${\\mathbb N}$ on a case-by-case basis, an impossible task if $S$ is an infinite set, we give a specific proof for the smallest integer being considered, followed by a generic argument showing that if the statement holds for a given case, then it must also hold for the next  case in the sequence.  We summarize mathematical induction in the following axiom.</p></div>"]},
{"cell_type":"markdown", "metadata":{}, "source":["<div class=\"mathbook-content\"><article class=\"theorem-like\"><a knowl=\"\" class=\"id-ref\" refid=\"hk-principle-1\" id=\"principle-1\"><h6 class=\"heading\"><span class=\"type\">Principle</span><span class=\"codenumber\">2.1.1</span><span class=\"title\">First Principle of Mathematical Induction</span></h6></a></article><div id=\"hk-principle-1\" class=\"hidden-content tex2jax_ignore\"><article class=\"theorem-like\"><p id=\"p-250\">Let $S(n)$ be a statement about integers for  $n \\in {\\mathbb N}$ and suppose $S(n_0)$ is true for some integer $n_0\\text{.}$  If for all integers $k$ with $k \\geq n_0\\text{,}$ $S(k)$ implies that $S(k+1)$ is true, then $S(n)$ is true for all integers $n$ greater than or equal to $n_0\\text{.}$</p></article></div></div>"]},
{"cell_type":"markdown", "metadata":{}, "source":["<div class=\"mathbook-content\"><article class=\"example-like\" id=\"example-integers-induction-greater-than\"><h6 class=\"heading\"><span class=\"type\">Example</span><span class=\"codenumber\">2.1.2</span><span class=\"title\">An inequality for powers of $2$</span></h6><p id=\"p-251\">For all integers $n \\geq 3\\text{,}$ $2^n \\gt n + 4\\text{.}$ Since</p><div class=\"displaymath\">\n\\begin{equation*}\n8 = 2^3 \\gt 3 + 4 = 7,\n\\end{equation*}\n</div><p>the statement is true for $n_0 = 3\\text{.}$  Assume that $2^k \\gt k + 4$ for $k \\geq 3\\text{.}$  Then $2^{k + 1} = 2 \\cdot 2^{k} \\gt 2(k + 4)\\text{.}$  But</p><div class=\"displaymath\">\n\\begin{equation*}\n2(k + 4) = 2k + 8 \\gt k + 5 = (k + 1) + 4\n\\end{equation*}\n</div><p>since $k$ is positive.  Hence, by induction, the statement holds for all integers $n \\geq 3\\text{.}$</p></article></div>"]},
{"cell_type":"markdown", "metadata":{}, "source":["<div class=\"mathbook-content\"><article class=\"example-like\" id=\"example-integers-induction-divisible\"><h6 class=\"heading\"><span class=\"type\">Example</span><span class=\"codenumber\">2.1.3</span><span class=\"title\">Some integers divisible by $9$</span></h6><p id=\"p-252\">Every integer $10^{n + 1} + 3 \\cdot 10^n + 5$ is divisible by 9 for $n \\in {\\mathbb N}\\text{.}$  For $n = 1\\text{,}$</p><div class=\"displaymath\">\n\\begin{equation*}\n10^{1 + 1} + 3 \\cdot 10 + 5 = 135 = 9 \\cdot 15\n\\end{equation*}\n</div><p>is divisible by 9.  Suppose that $10^{k + 1} + 3 \\cdot 10^k + 5$ is divisible by 9 for $k \\geq 1\\text{.}$  Then</p><div class=\"displaymath\">\n\\begin{align*}\n10^{(k + 1) + 1} + 3 \\cdot 10^{k + 1} + 5& = 10^{k + 2} + 3 \\cdot 10^{k + 1} + 50 - 45\\\\\n& = 10 (10^{k + 1} + 3 \\cdot 10^{k} + 5) - 45\n\\end{align*}\n</div><p>is divisible by 9.</p></article></div>"]},
{"cell_type":"markdown", "metadata":{}, "source":["<div class=\"mathbook-content\"><article class=\"example-like\" id=\"example-integers-binomial-theorem\"><h6 class=\"heading\"><span class=\"type\">Example</span><span class=\"codenumber\">2.1.4</span><span class=\"title\">The binomial theorem</span></h6><p id=\"p-253\">We will prove the binomial theorem using mathematical induction; that is,</p><div class=\"displaymath\">\n\\begin{equation*}\n(a + b)^n = \\sum_{k = 0}^{n} \\binom{n}{k} a^k b^{n - k},\n\\end{equation*}\n</div><p>where $a$ and $b$ are real numbers, $n \\in \\mathbb{N}\\text{,}$ and</p><div class=\"displaymath\">\n\\begin{equation*}\n\\binom{n}{k} = \\frac{n!}{k! (n - k)!}\n\\end{equation*}\n</div><p>is the binomial coefficient.  We first show that</p><div class=\"displaymath\">\n\\begin{equation*}\n\\binom{n + 1}{k} = \\binom{n}{k} + \\binom{n}{k - 1}.\n\\end{equation*}\n</div><p>This result follows from</p><div class=\"displaymath\">\n\\begin{align*}\n\\binom{n}{k} + \\binom{n}{k - 1} & = \\frac{n!}{k!(n - k)!} +\\frac{n!}{(k-1)!(n - k + 1)!}\\\\\n& = \\frac{(n + 1)!}{k!(n + 1 - k)!}\\\\\n& =\\binom{n + 1}{k}.\n\\end{align*}\n</div><p id=\"p-254\">If $n = 1\\text{,}$ the binomial theorem is easy to verify. Now assume that the result is true for $n$ greater than or equal to 1.  Then</p><div class=\"displaymath\">\n\\begin{align*}\n(a + b)^{n + 1} & = (a + b)(a + b)^n\\\\\n& = (a + b) \\left( \\sum_{k = 0}^{n} \\binom{n}{k} a^k b^{n - k}\\right)\\\\\n& = \\sum_{k = 0}^{n} \\binom{n}{k} a^{k + 1} b^{n - k} + \\sum_{k = 0}^{n} \\binom{n}{k} a^k b^{n + 1 - k}\\\\\n& = a^{n + 1} + \\sum_{k = 1}^{n} \\binom{n}{k - 1} a^{k} b^{n + 1 - k} + \\sum_{k = 1}^{n} \\binom{n}{k}  a^k b^{n + 1 - k} + b^{n + 1}\\\\\n&  = a^{n + 1} + \\sum_{k = 1}^{n} \\left[ \\binom{n}{k - 1} + \\binom{n}{k} \\right]a^k b^{n + 1 - k} + b^{n + 1}\\\\\n&  = \\sum_{k = 0}^{n + 1}   \\binom{n + 1}{k} a^k b^{n + 1- k}.\n\\end{align*}\n</div></article></div>"]},
{"cell_type":"markdown", "metadata":{}, "source":["<div class=\"mathbook-content\"><p id=\"p-255\">We have an equivalent statement of the Principle of Mathematical Induction that is often very useful.</p></div>"]},
{"cell_type":"markdown", "metadata":{}, "source":["<div class=\"mathbook-content\"><article class=\"theorem-like\"><a knowl=\"\" class=\"id-ref\" refid=\"hk-principle-2\" id=\"principle-2\"><h6 class=\"heading\"><span class=\"type\">Principle</span><span class=\"codenumber\">2.1.5</span><span class=\"title\">Second Principle of Mathematical Induction</span></h6></a></article><div id=\"hk-principle-2\" class=\"hidden-content tex2jax_ignore\"><article class=\"theorem-like\"><p id=\"p-256\">Let $S(n)$ be a statement about integers for  $n \\in {\\mathbb N}$ and suppose $S(n_0)$ is true for some integer $n_0\\text{.}$  If $S(n_0), S(n_0 + 1), \\ldots, S(k)$ imply that $S(k + 1)$ for $k \\geq n_0\\text{,}$ then the statement $S(n)$ is true for all integers $n \\geq n_0\\text{.}$</p></article></div></div>"]},
{"cell_type":"markdown", "metadata":{}, "source":["<div class=\"mathbook-content\"><p id=\"p-257\">A  nonempty subset $S$ of ${\\mathbb Z}$ is <dfn class=\"terminology\">well-ordered</dfn> if $S$ contains a least element.  Notice that the set ${\\mathbb Z}$ is not well-ordered since it does not contain a smallest element.  However, the natural numbers are well-ordered.</p></div>"]},
{"cell_type":"markdown", "metadata":{}, "source":["<div class=\"mathbook-content\"><article class=\"theorem-like\"><a knowl=\"\" class=\"id-ref\" refid=\"hk-principle-3\" id=\"principle-3\"><h6 class=\"heading\"><span class=\"type\">Principle</span><span class=\"codenumber\">2.1.6</span><span class=\"title\">Principle of Well-Ordering</span></h6></a></article><div id=\"hk-principle-3\" class=\"hidden-content tex2jax_ignore\"><article class=\"theorem-like\"><p id=\"p-258\">Every nonempty subset of the natural numbers is well-ordered.</p></article></div></div>"]},
{"cell_type":"markdown", "metadata":{}, "source":["<div class=\"mathbook-content\"><p id=\"p-259\">The Principle of Well-Ordering is equivalent to the Principle of Mathematical Induction.</p></div>"]},
{"cell_type":"markdown", "metadata":{}, "source":["<div class=\"mathbook-content\"><article class=\"theorem-like\"><a knowl=\"\" class=\"id-ref\" refid=\"hk-lemma-integers-smallest-number\" id=\"lemma-integers-smallest-number\"><h6 class=\"heading\"><span class=\"type\">Lemma</span><span class=\"codenumber\">2.1.7</span></h6></a></article><div id=\"hk-lemma-integers-smallest-number\" class=\"hidden-content tex2jax_ignore\"><article class=\"theorem-like\"><p id=\"p-260\">The Principle of Mathematical Induction implies that $1$ is the least positive natural number.</p></article><article class=\"proof\" id=\"proof-6\"><h6 class=\"heading\"><span class=\"type\">Proof</span></h6><p id=\"p-261\">Let $S = \\{ n \\in {\\mathbb N} : n \\geq 1 \\}\\text{.}$ Then $1 \\in S\\text{.}$  Now assume that $n \\in S\\text{;}$ that is, $n \\geq 1\\text{.}$  Since $n+1 \\geq 1\\text{,}$ $n+ 1 \\in S\\text{;}$ hence, by induction, every natural number is greater than or equal to 1.</p></article></div></div>"]},
{"cell_type":"markdown", "metadata":{}, "source":["<div class=\"mathbook-content\"><article class=\"theorem-like\"><a knowl=\"\" class=\"id-ref\" refid=\"hk-theorem-integers-pmi-implies-pwo\" id=\"theorem-integers-pmi-implies-pwo\"><h6 class=\"heading\"><span class=\"type\">Theorem</span><span class=\"codenumber\">2.1.8</span></h6></a></article><div id=\"hk-theorem-integers-pmi-implies-pwo\" class=\"hidden-content tex2jax_ignore\"><article class=\"theorem-like\"><p id=\"p-262\">The Principle of Mathematical Induction implies the Principle of Well-Ordering.  That is, every nonempty subset of $\\mathbb N$ contains a least element.</p></article><article class=\"proof\" id=\"proof-7\"><h6 class=\"heading\"><span class=\"type\">Proof</span></h6><p id=\"p-263\">We must show that if $S$ is a nonempty subset of the natural numbers, then $S$ contains a least element.  If $S$ contains 1, then the theorem is true by LemmaÂ <a href=\"section-math-induction.ipynb#lemma-integers-smallest-number\" class=\"xref\" alt=\"Lemma 2.1.7 \" title=\"Lemma 2.1.7 \">LemmaÂ 2.1.7</a>.  Assume that if $S$ contains an integer $k$ such that $1 \\leq k \\leq n\\text{,}$ then $S$ contains a least element.  We will show that if a set $S$ contains an integer less than or equal to $n + 1\\text{,}$ then $S$ has a least element.  If $S$ does not contain an integer less than $n+1\\text{,}$ then $n+1$ is the smallest integer in $S\\text{.}$  Otherwise, since $S$ is nonempty, $S$ must contain an integer less than or equal to $n\\text{.}$ In this case, by induction, $S$ contains a least element.</p></article></div></div>"]},
{"cell_type":"markdown", "metadata":{}, "source":["<div class=\"mathbook-content\"><p id=\"p-264\">Induction can also be very useful in formulating definitions. For instance, there are two ways to define $n!\\text{,}$ the factorial of a positive integer $n\\text{.}$</p><ul class=\"disc\"><li id=\"li-70\"><p id=\"p-265\">The <em class=\"emphasis\">explicit</em> definition: $n! = 1 \\cdot 2 \\cdot 3 \\cdots (n - 1) \\cdot n\\text{.}$</p></li><li id=\"li-71\"><p id=\"p-266\">The <em class=\"emphasis\">inductive</em> or <em class=\"emphasis\">recursive</em> definition: $1! = 1$ and $n! = n(n - 1)!$ for $n \\gt 1\\text{.}$</p></li></ul></div>"]},
{"cell_type":"markdown", "metadata":{}, "source":["<div class=\"mathbook-content\"><p id=\"p-267\">Every good mathematician or computer scientist knows that looking at problems recursively, as opposed to explicitly, often results in better understanding of complex issues.</p></div>"]}
],
"nbformat": 4, "nbformat_minor": 0, "metadata": {"kernelspec": {"display_name": "", "name": "python3"}, "language_info": {"codemirror_mode": {"name": "ipython", "version": 2}, "file_extension": ".py", "mimetype": "text/x-python", "name": "python", "nbconvert_exporter": "python", "pygments_lexer": "ipython2", "version": "2.7.8"}, "name": "section-math-induction.ipynb"}
}